RAC of memory properties: full syntax

Memory/Syntax.v
@@ -5,15 +5,17 @@ Require Import Vrac.MemoryType Vrac.Error Vrac.Option Vrac.Tactics.
 
 Module Syntax(V : DecidableType).
 
+  Open Scope error_monad_scope.
+  
   Module Types.
   
-    Inductive type :=
-    | TInt : Mtyp.t -> type
-    | TPtr: type -> type.
+    Inductive ctyp :=
+    | TInt : Mtyp.t -> ctyp
+    | TPtr: ctyp -> ctyp.
 
-    Definition t := type.
+    Definition t := ctyp.
     
-    Definition mtype: mtyp -> type -> mtyp :=
+    Definition mtype: mtyp -> ctyp -> mtyp :=
       fun machine_word ty =>
         match ty with
         | TInt mtype => mtype 
@@ -48,87 +50,261 @@ Module Syntax(V : DecidableType).
   
   Module T := Eqb.Full Types. Import Types. Import T.
 
-  Ltac simpl_type_eqb :=
+  Ltac simpl_ctyp_eqb :=
     simpl_generic_eqb eqb eqb_refl eqb_sym eqb_eq eqb_neq.
-  
-  Inductive unary_operation : Type :=
-  | Onot
-  | Oneg.
-  
-  Inductive binary_operation : Type :=
-  | Oadd  (* addition *)
-  | Osub  (* subtraction *)
-  | Omul  (* multiplication *)
-  | Odiv  (* division *)
-  | Omod  (* remainder *)
-  | Oeq   (* comparison (==) *)
-  | Olt   (* comparison (<) *)
-  | Ogt   (* comparison (>) *)
-  | Ole   (* comparison (<=) *)
-  | Oge   (* comparison (>=) *).
 
-  Inductive expr : Type :=
-  | EInt (n: Z) (τ: type)      (* Integer value *)
-  | EVar (x: V.t) (τ: type)    (* variable *)
-  | EDeref (e: expr) (τ: type) (* dereference *)
-  | EAddrof (e: expr) (τ: type)(* address *)
-  | EUnop (op: unary_operation) (e: expr) (τ: type)
-  | EBinop (op: binary_operation) (e1 e2: expr) (τ: type).
 
-  Definition type_int (n:Z) (τ:type) : result type :=
+  Definition match_ctyp τ τ' : result ctyp :=
+    if Types.eqb τ τ'
+    then Ok τ
+    else Error "type mismatch".
+  
+  Definition type_int (n:Z) (τ:ctyp) : result ctyp :=
     match τ with
     | TInt κ =>  if ( (min_int (sizeof κ)<=? n)%Z &&
-                     (n <=? max_int (sizeof κ))%Z )%bool
+                       (n <=? max_int (sizeof κ))%Z )%bool
                 then Ok τ
                 else Error "not storable"
     | _ => Error "not an integer type"
     end.
 
-  Open Scope error_monad_scope.
-
-  Definition same_as_checked τ τ' : result type :=
-     if Types.eqb τ τ'
-     then Ok τ
-     else Error "type mismatch".
-
-  Definition type_env := V.t -> option type.
+  Definition type_env := V.t -> option ctyp.
   
-  Fixpoint check_type (Γ: type_env) (e: expr) : result type :=
-    match e with
-    | EInt n τ => type_int n τ
-    | EVar x τ => match Γ x with
-                 | ϵ => Error "undefined identifier"
-                 | ⎣τ'⎦ => same_as_checked τ τ'
-                 end
-    | EDeref e τ =>
-        match check_type Γ e with 
-        | Ok (TPtr τ') => same_as_checked τ τ'
-        | _ => Error "not dereferencing a pointer"
-        end
-    | EAddrof e τ =>
-        do τ' <- check_type Γ e;
-        same_as_checked τ (TPtr τ')
-    | EUnop op e τ =>
-        do τ' <- check_type Γ e;
-        match τ' with
-        | TInt _ => same_as_checked τ τ'
-        | TPtr _ => Error "no unary operation on pointers"
-        end
-    | EBinop op e1 e2 τ =>
-        do τ1 <- check_type Γ e1;
-        do τ2 <- check_type Γ e2;
-        match (op, τ1, τ2) with
-        | (_, TInt κ1, TInt κ2) =>
-            same_as_checked τ (TInt (MemoryType.max κ1 κ2))
-        | ((Oadd|Osub), TPtr τ', TInt _) =>
-            same_as_checked τ (TPtr τ')
-        | (Oeq, TPtr τ'1, TPtr τ'2) =>
-            if Types.eqb τ'1 τ'2
-            then same_as_checked τ (TInt i8)
-            else Error "incompatible types for eq"
-        | _ => Error "incorrect types for binary operation"
-        end
-    end.
+  Module Expr.
+  
+    Inductive unary_operation : Type :=
+    | Onot
+    | Oneg.
+    
+    Inductive binary_operation : Type :=
+    | Oadd  (* addition *)
+    | Osub  (* subtraction *)
+    | Omul  (* multiplication *)
+    | Odiv  (* division *)
+    | Omod  (* remainder *)
+    | Oeq   (* comparison (==) *)
+    | Olt   (* comparison (<) *)
+    | Ogt   (* comparison (>) *)
+    | Ole   (* comparison (<=) *)
+    | Oge   (* comparison (>=) *).
+    
+    Inductive expr : Type :=
+    | EInt (n: Z) (τ: ctyp)      (* Integer value *)
+    | EVar (x: V.t) (τ: ctyp)    (* variable *)
+    | EDeref (e: expr) (τ: ctyp) (* dereference *)
+    | EAddrof (e: expr) (τ: ctyp)(* address *)
+    | EUnop (op: unary_operation) (e: expr) (τ: ctyp)
+    | EBinop (op: binary_operation) (e1 e2: expr) (τ: ctyp).
+        
+    Fixpoint check_type (Γ: type_env) (e: expr) : result ctyp :=
+      match e with
+      | EInt n τ => type_int n τ
+      | EVar x τ => match Γ x with
+                   | ϵ => Error "undefined identifier"
+                   | ⎣τ'⎦ => match_ctyp τ τ'
+                   end
+      | EDeref e τ =>
+          match check_type Γ e with 
+          | Ok (TPtr τ') => match_ctyp τ τ'
+          | _ => Error "not dereferencing a pointer"
+          end
+      | EAddrof e τ =>
+          do τ' <- check_type Γ e;
+          match_ctyp τ (TPtr τ')
+      | EUnop op e τ =>
+          do τ' <- check_type Γ e;
+          match τ' with
+          | TInt _ => match_ctyp τ τ'
+          | TPtr _ => Error "no unary operation on pointers"
+          end
+      | EBinop op e1 e2 τ =>
+          do τ1 <- check_type Γ e1;
+          do τ2 <- check_type Γ e2;
+          match (op, τ1, τ2) with
+          | (_, TInt κ1, TInt κ2) =>
+              match_ctyp τ (TInt (MemoryType.max κ1 κ2))
+          | ((Oadd|Osub), TPtr τ', TInt _) =>
+              match_ctyp τ (TPtr τ')
+          | (Oeq, TPtr τ'1, TPtr τ'2) =>
+              if Types.eqb τ'1 τ'2
+              then match_ctyp τ (TInt i8)
+              else Error "incompatible types for eq"
+          | _ => Error "incorrect types for binary operation"
+          end
+      end.
+
+  End Expr.
+
+  Import Expr.
+
+  Module Term.
+    
+    Inductive term :=
+    | TExpr (e: expr) (τ: ctyp)
+    | TDeref (t: term) (τ: ctyp)
+    | TUnop (op: unary_operation) (t: term) (τ: ctyp)
+    | TBinop (op: binary_operation) (t1: term) (t2: term) (τ: ctyp)
+    | TBaseaddress (t: term) (τ: ctyp)
+    | TOffset (t: term) (τ: ctyp)
+    | TBlocklength (t: term) (τ: ctyp).
+
+    Fixpoint check_type (Γ: type_env) (t: term) : result ctyp :=
+      match t with
+      | TExpr e τ => Expr.check_type Γ e
+      | TDeref t τ =>
+          match check_type Γ t with 
+          | Ok (TPtr τ') => match_ctyp τ τ'
+          | _ => Error "not dereferencing a pointer"
+          end
+      | TUnop op t τ =>
+          do τ' <- check_type Γ t;
+          match τ' with
+          | TInt _ => match_ctyp τ τ'
+          | TPtr _ => Error "no unary operation on pointers"
+          end
+      | TBinop op t1 t2 τ =>
+          do τ1 <- check_type Γ t1;
+          do τ2 <- check_type Γ t2;
+          match (op, τ1, τ2) with
+          | (_, TInt κ1, TInt κ2) =>
+              match_ctyp τ (TInt (MemoryType.max κ1 κ2))
+          | ((Oadd|Osub), TPtr τ', TInt _) =>
+              match_ctyp τ (TPtr τ')
+          | (Oeq, TPtr τ'1, TPtr τ'2) =>
+              if Types.eqb τ'1 τ'2
+              then match_ctyp τ (TInt i8)
+              else Error "incompatible types for eq"
+          | _ => Error "incorrect types for binary operation"
+          end
+      | TBaseaddress t τ =>
+          do τ' <- check_type Γ t;
+          match_ctyp τ (TPtr τ')
+      | TOffset t τ =>
+          do τ' <- check_type Γ t;
+          match (τ', τ) with
+          | (TPtr _, TInt _) => Ok τ
+          | (TPtr _, _) => Error "offset should be an integer"
+          | (_, _) => Error "argument of offset should be a pointer"
+          end
+      | TBlocklength t τ =>
+          do τ' <- check_type Γ t;
+          match (τ', τ) with
+          | (TPtr _, TInt _) => Ok τ
+          | (TPtr _, _) => Error "block_length should be an integer"
+          | (_, _) => Error "argument of block_length should be a pointer"
+          end
+      end.
+    
+  End Term.
+
+  Import Term.
+  
+  Module Pred.
+
+    Inductive relational_predicate :=
+    | PEq
+    | PLt
+    | PGt
+    | PLe
+    | PGe.
+    
+    Inductive pred :=
+    | PTrue
+    | PFalse
+    | PComp (R: relational_predicate) (t1 t2: term)
+    | PAnd (p1 p2: pred)
+    | PNot (p: pred)
+    | PValid (t: term)
+    | PInitialized (t: term).
+
+    Fixpoint check_type Γ p : result unit :=
+      match p with
+      | PTrue | PFalse => Ok tt
+      | PComp R t1 t2 =>
+          do τ1 <- Term.check_type Γ t1;
+          do τ2 <- Term.check_type Γ t2;
+          match (R, τ1, τ2) with
+          | (_, TInt _, TInt _) => Ok tt
+          | (PEq, TPtr τ'1, TPtr τ'2) =>
+              if Types.eqb τ'1 τ'2
+              then Ok tt
+              else Error "incompatible types for equality"
+          | _ => Error "incorrect types for comparison"
+          end
+      | PNot p => check_type Γ p
+      | PAnd p1 p2 =>
+          do ct1 <- check_type Γ p1;
+          do ct2 <- check_type Γ p2;
+          Ok tt
+      | (PValid t | PInitialized t) =>
+          do τ' <- Term.check_type Γ t;
+          match τ' with
+          | TPtr _ => Ok tt
+          | _ => Error "argument of valid should be a pointer term"
+          end
+      end%bool.
+
+  End Pred.
+
+  Import Pred.
+
+  Module Stmt.
+
+    Inductive stmt :=
+    | SSkip
+    | SAssign (e1 e2: expr)
+    | SSeq (s1 s2: stmt)
+    | SIf (e: expr) (s1 s2: stmt)
+    | SWhile (e: expr) (s: stmt)
+    | SMalloc (e1 e2: expr)
+    | SFree (e: expr)
+    | SLet (x: V.t)(τ: ctyp)(s: stmt)
+    | SLogicalassert (p: pred).
+
+    Fixpoint check_type Γ (s: stmt) : result unit :=
+      match s with
+      | SSkip => Ok tt
+      | SAssign e1 e2 =>
+          do τ1 <- Expr.check_type Γ e1;
+          do τ2 <- Expr.check_type Γ e2;
+          do r <- match_ctyp τ1 τ2;
+          Ok tt
+      | SSeq s1 s2 =>
+          do ct1 <- check_type Γ s1;
+          do ct2 <- check_type Γ s2;
+          Ok tt
+      | SIf e s1 s2 =>
+          do τ <- Expr.check_type Γ e;
+          do ct1 <- check_type Γ s1;
+          do ct2 <- check_type Γ s2;
+          Ok tt
+      | SWhile e s =>
+          do τ <- Expr.check_type Γ e;
+          do ct <- check_type Γ s;
+          Ok tt                     
+      | SMalloc e1 e2 =>
+          do τ1 <- Expr.check_type Γ e1;
+          do τ2 <- Expr.check_type Γ e2;
+          match (τ1, τ2) with
+          | (TPtr _, TInt _) => Ok tt
+          | _ => Error "incorrect types for malloc"
+          end
+      | SFree e =>
+          do τ <- Expr.check_type Γ e;
+          match τ with
+          | TPtr _ => Ok tt
+          | _ => Error "incorrect type for free"
+          end
+      | SLet x τ s =>
+          let Γ' := fun y => if V.eq_dec y x then ⎣τ⎦ else Γ y in
+          check_type Γ' s
+      | SLogicalassert p =>
+          Pred.check_type Γ p
+      end.
+
+  End Stmt.
+    
+  Close Scope error_monad_scope.
   
 End Syntax.
 
